theories/tree_borrows/steps_preserve.v
@@ -106,21 +106,21 @@ Lemma apply_access_spec_per_node
   {tr affected_tag access_tag pre fn cids range tr'}
   (*(ExAcc : tree_contains access_tag tr)*)
   (ExAff : tree_contains affected_tag tr)
-  (UnqAff : tree_unique affected_tag pre tr)
+  (UnqAff : tree_item_determined affected_tag pre tr)
   (Access : tree_apply_access fn cids access_tag range tr = Some tr')
   : exists post,
     Some post = item_apply_access fn cids (rel_dec tr access_tag pre.(itag)) range pre
     /\ tree_contains affected_tag tr'
-    /\ tree_unique affected_tag post tr'.
+    /\ tree_item_determined affected_tag post tr'.
 Proof.
   (* Grab the success condition of every node separately *)
   pose proof (proj1 (join_success_condition _) (mk_is_Some _ _ Access)) as SuccessCond.
   rewrite every_node_map in SuccessCond; rewrite every_node_eqv_universal in SuccessCond.
-  pose proof (exists_unique_exists _ _ _ ExAff UnqAff) as Expre.
+  pose proof (exists_determined_exists _ _ _ ExAff UnqAff) as Expre.
   pose proof (SuccessCond pre Expre) as [post SpecPost].
-  unfold tree_unique in UnqAff. rewrite every_node_eqv_universal in UnqAff.
+  unfold tree_item_determined in UnqAff. rewrite every_node_eqv_universal in UnqAff.
   (* Now do some transformations to get to the node level *)
-  unfold tree_unique.
+  unfold tree_item_determined.
   exists post.
   split; [symmetry; auto|].
   split; [rewrite <- (access_preserves_tags Access); exact ExAff|].
@@ -163,30 +163,30 @@ Proof.
     eapply insertion_preserves_tags; eauto.
 Qed.
 
-Lemma bor_local_step_retag_produces_contains_unique
+Lemma bor_local_step_retag_produces_contains_determined
   {tgp tg tr tr' cids cids' newp cid}
   (Step : bor_local_step
     tr cids
     (RetagBLEvt tgp tg newp cid)
     tr' cids')
   : tree_contains tg tr'
-  /\ tree_unique tg (create_new_item tg newp) tr'.
+  /\ tree_item_determined tg (create_new_item tg newp) tr'.
 Proof.
   inversion Step as [| | |????????? RETAG_EFFECT]; subst.
   split.
   - eapply insertion_contains; eauto.
   - injection RETAG_EFFECT; intros; subst.
-    eapply inserted_unique; [apply new_item_has_tag|].
+    eapply inserted_determined; [apply new_item_has_tag|].
     assumption.
 Qed.
 
-Lemma bor_local_step_preserves_unique_easy
+Lemma bor_local_step_preserves_determined_easy
   {tg tr it tr' cids cids' evt}
   (Ex : tree_contains tg tr)
-  (Unq : tree_unique tg it tr)
+  (Unq : tree_item_determined tg it tr)
   (Step : bor_local_step tr cids evt tr' cids')
   : exists it',
-  tree_unique tg it' tr'
+  tree_item_determined tg it' tr'
   /\ match evt with
   | AccessBLEvt _ _ _ => iprot it = iprot it'
   | InitCallBLEvt _
@@ -204,7 +204,7 @@ Proof.
   - eexists; split; [|reflexivity]; assumption.
   - (* Retag *)
     eexists; split; [|reflexivity].
-    eapply create_child_preserves_unique; [|exact Unq|exact RETAG_EFFECT].
+    eapply create_child_preserves_determined; [|exact Unq|exact RETAG_EFFECT].
     intro; subst. destruct (FRESH_CHILD Ex).
 Qed.
 
@@ -301,14 +301,14 @@ Qed.
 Lemma memory_access_preserves_backward_reach
   {access_tag affected_tag pre tr post tr' kind cids range p0 z}
   (ExAff : tree_contains affected_tag tr)
-  (UnqAff : tree_unique affected_tag pre tr)
+  (UnqAff : tree_item_determined affected_tag pre tr)
   (ExAcc : tree_contains access_tag tr)
   (Access : memory_access kind cids access_tag range tr = Some tr')
-  (UnqAff' : tree_unique affected_tag post tr')
+  (UnqAff' : tree_item_determined affected_tag post tr')
   : reach p0 (item_perm_at_loc pre z) -> reach p0 (item_perm_at_loc post z).
 Proof.
   destruct (apply_access_spec_per_node ExAff UnqAff Access) as [post' [PostSpec [ExPost UnqPost]]].
-  pose proof (tree_unique_unify ExPost UnqPost UnqAff'); subst.
+  pose proof (tree_determined_unify ExPost UnqPost UnqAff'); subst.
   (* now it's just bruteforce case analysis *)
   generalize dependent post.
   generalize dependent pre.
@@ -327,14 +327,14 @@ Qed.
 Lemma memory_access_preserves_forward_unreach
   {access_tag affected_tag pre tr post tr' kind cids range p0 z}
   (ExAff : tree_contains affected_tag tr)
-  (UnqAff : tree_unique affected_tag pre tr)
+  (UnqAff : tree_item_determined affected_tag pre tr)
   (ExAcc : tree_contains access_tag tr)
   (Access : memory_access kind cids access_tag range tr = Some tr')
-  (UnqAff' : tree_unique affected_tag post tr')
+  (UnqAff' : tree_item_determined affected_tag post tr')
   : ~reach (item_perm_at_loc pre z) p0 -> ~reach (item_perm_at_loc post z) p0.
 Proof.
   destruct (apply_access_spec_per_node ExAff UnqAff Access) as [post' [PostSpec [ExPost UnqPost]]].
-  pose proof (tree_unique_unify ExPost UnqPost UnqAff'); subst.
+  pose proof (tree_determined_unify ExPost UnqPost UnqAff'); subst.
   (* now it's just bruteforce case analysis *)
   generalize dependent post.
   generalize dependent pre.
@@ -353,15 +353,15 @@ Qed.
 Lemma memory_access_preserves_protected_freeze_like
   {access_tag affected_tag pre tr post tr' kind cids range z}
   (ExAff : tree_contains affected_tag tr)
-  (UnqAff : tree_unique affected_tag pre tr)
+  (UnqAff : tree_item_determined affected_tag pre tr)
   (ExAcc : tree_contains access_tag tr)
   (Prot : protector_is_active (iprot pre) cids)
   (Access : memory_access kind cids access_tag range tr = Some tr')
-  (UnqAff' : tree_unique affected_tag post tr')
+  (UnqAff' : tree_item_determined affected_tag post tr')
   : freeze_like (item_perm_at_loc pre z) -> freeze_like (item_perm_at_loc post z).
 Proof.
   destruct (apply_access_spec_per_node ExAff UnqAff Access) as [post' [PostSpec [ExPost UnqPost]]].
-  pose proof (tree_unique_unify ExPost UnqPost UnqAff'); subst.
+  pose proof (tree_determined_unify ExPost UnqPost UnqAff'); subst.
   (* now it's just bruteforce case analysis *)
   generalize dependent post.
   generalize dependent pre.
@@ -381,53 +381,53 @@ Qed.
 Lemma bor_local_step_preserves_backward_reach
   {tg tr tr' cids cids' pre post evt p0 z}
   (Ex : tree_contains tg tr)
-  (UnqPre : tree_unique tg pre tr)
+  (UnqPre : tree_item_determined tg pre tr)
   (Step : bor_local_step tr cids evt tr' cids')
-  (UnqPost : tree_unique tg post tr')
+  (UnqPost : tree_item_determined tg post tr')
   : reach p0 (item_perm_at_loc pre z) -> reach p0 (item_perm_at_loc post z).
 Proof.
   inversion Step as [???? EXISTS_TAG ACC| | |]; subst.
   - apply (memory_access_preserves_backward_reach Ex UnqPre EXISTS_TAG ACC UnqPost).
-  - rewrite (tree_unique_unify Ex UnqPre UnqPost); tauto.
-  - rewrite (tree_unique_unify Ex UnqPre UnqPost); tauto.
+  - rewrite (tree_determined_unify Ex UnqPre UnqPost); tauto.
+  - rewrite (tree_determined_unify Ex UnqPre UnqPost); tauto.
   - pose proof (bor_local_step_preserves_contains Ex Step) as ExPost'.
-    pose proof (bor_local_step_preserves_unique_easy Ex UnqPre Step) as [it' [UnqPost' Eq]]; subst; simpl in UnqPost'.
-    rewrite (tree_unique_unify ExPost' UnqPost' UnqPost); tauto.
+    pose proof (bor_local_step_preserves_determined_easy Ex UnqPre Step) as [it' [UnqPost' Eq]]; subst; simpl in UnqPost'.
+    rewrite (tree_determined_unify ExPost' UnqPost' UnqPost); tauto.
 Qed.
 
 Lemma bor_local_step_preserves_forward_unreach
   {tg tr tr' cids cids' pre post evt p0 z}
   (Ex : tree_contains tg tr)
-  (UnqPre : tree_unique tg pre tr)
+  (UnqPre : tree_item_determined tg pre tr)
   (Step : bor_local_step tr cids evt tr' cids')
-  (UnqPost : tree_unique tg post tr')
+  (UnqPost : tree_item_determined tg post tr')
   : ~reach (item_perm_at_loc pre z) p0 -> ~reach (item_perm_at_loc post z) p0.
 Proof.
   inversion Step as [???? EXISTS_TAG ACC| | |]; subst.
   - apply (memory_access_preserves_forward_unreach Ex UnqPre EXISTS_TAG ACC UnqPost).
-  - rewrite (tree_unique_unify Ex UnqPre UnqPost); tauto.
-  - rewrite (tree_unique_unify Ex UnqPre UnqPost); tauto.
+  - rewrite (tree_determined_unify Ex UnqPre UnqPost); tauto.
+  - rewrite (tree_determined_unify Ex UnqPre UnqPost); tauto.
   - pose proof (bor_local_step_preserves_contains Ex Step) as ExPost'.
-    pose proof (bor_local_step_preserves_unique_easy Ex UnqPre Step) as [it' [UnqPost' Eq]]; subst; simpl in UnqPost'.
-    rewrite (tree_unique_unify ExPost' UnqPost' UnqPost); tauto.
+    pose proof (bor_local_step_preserves_determined_easy Ex UnqPre Step) as [it' [UnqPost' Eq]]; subst; simpl in UnqPost'.
+    rewrite (tree_determined_unify ExPost' UnqPost' UnqPost); tauto.
 Qed.
 
 Lemma bor_local_step_preserves_protected_freeze_like
   {tg tr tr' cids cids' pre post evt z}
   (Ex : tree_contains tg tr)
-  (UnqPre : tree_unique tg pre tr)
+  (UnqPre : tree_item_determined tg pre tr)
   (Prot : protector_is_active (iprot pre) cids)
   (Step : bor_local_step tr cids evt tr' cids')
-  (UnqPost : tree_unique tg post tr')
+  (UnqPost : tree_item_determined tg post tr')
   : freeze_like (item_perm_at_loc pre z) -> freeze_like (item_perm_at_loc post z).
 Proof.
   inversion Step as [???? EXISTS_TAG ACC| | |]; subst.
   - apply (memory_access_preserves_protected_freeze_like Ex UnqPre EXISTS_TAG Prot ACC UnqPost).
-  - rewrite (tree_unique_unify Ex UnqPre UnqPost); tauto.
-  - rewrite (tree_unique_unify Ex UnqPre UnqPost); tauto.
+  - rewrite (tree_determined_unify Ex UnqPre UnqPost); tauto.
+  - rewrite (tree_determined_unify Ex UnqPre UnqPost); tauto.
   - pose proof (bor_local_step_preserves_contains Ex Step) as ExPost'.
-    pose proof (bor_local_step_preserves_unique_easy Ex UnqPre Step) as [it' [UnqPost' Eq]]; subst; simpl in UnqPost'.
-    rewrite (tree_unique_unify ExPost' UnqPost' UnqPost); tauto.
+    pose proof (bor_local_step_preserves_determined_easy Ex UnqPre Step) as [it' [UnqPost' Eq]]; subst; simpl in UnqPost'.
+    rewrite (tree_determined_unify ExPost' UnqPost' UnqPost); tauto.
 Qed.
 
 Lemma seq_always_build_forward
@@ -580,32 +580,32 @@ Proof.
   assumption.
 Qed.
 
-Lemma bor_local_seq_always_unique
+Lemma bor_local_seq_always_determined
   {tg tr tr' prot cids cids' evts pre}
   (Ex : tree_contains tg tr)
-  (Unq : tree_unique tg pre tr)
+  (Unq : tree_item_determined tg pre tr)
   (ProtEq : iprot pre = prot)
   (Seq : bor_local_seq {|seq_inv:=fun tr _ => (tree_contains tg) tr|} tr cids evts tr' cids')
-  : bor_local_seq {|seq_inv:=fun tr _ => exists it, tree_unique tg it tr /\ iprot it = prot|} tr cids evts tr' cids'.
+  : bor_local_seq {|seq_inv:=fun tr _ => exists it, tree_item_determined tg it tr /\ iprot it = prot|} tr cids evts tr' cids'.
 Proof.
   eapply seq_always_build_forward; [| |exact Seq].
   - eexists; split; eassumption.
   - clear. simpl. move=> ???? evt Step Ex [?[Unq Prot]].
-    destruct (bor_local_step_preserves_unique_easy Ex Unq Step) as [?[??]].
+    destruct (bor_local_step_preserves_determined_easy Ex Unq Step) as [?[??]].
     eexists.
     split; [eassumption|].
     destruct evt; subst; auto.
 Qed.
 
-Lemma bor_local_seq_last_unique
+Lemma bor_local_seq_last_determined
   {tg tr tr' cids cids' evts pre}
   (Ex : tree_contains tg tr)
-  (Unq : tree_unique tg pre tr)
+  (Unq : tree_item_determined tg pre tr)
   (Seq : bor_local_seq {|seq_inv:=fun _ _ => True|} tr cids evts tr' cids')
-  : exists post, tree_unique tg post tr' /\ iprot pre = iprot post.
+  : exists post, tree_item_determined tg post tr' /\ iprot pre = iprot post.
 Proof.
   pose proof (bor_local_seq_always_contains Ex Seq) as AllEx.
-  destruct (seq_always_destruct_last (bor_local_seq_always_unique Ex Unq eq_refl AllEx)) as [?[??]].
+  destruct (seq_always_destruct_last (bor_local_seq_always_determined Ex Unq eq_refl AllEx)) as [?[??]].
   eexists; split; subst; eauto.
 Qed.
 
@@ -661,16 +661,16 @@ Qed.
 Lemma bor_local_seq_always_backward_reach
   {tg tr tr' cids cids' pre evts p0 z}
   (Ex : tree_contains tg tr)
-  (Unq : tree_unique tg pre tr)
+  (Unq : tree_item_determined tg pre tr)
   (Reach : reach p0 (item_perm_at_loc pre z))
   (Seq : bor_local_seq {|seq_inv:=fun _ _ => True|} tr cids evts tr' cids')
-  : bor_local_seq {|seq_inv:=fun tr _ => forall post (UnqPost : tree_unique tg post tr), reach p0 (item_perm_at_loc post z)|}
+  : bor_local_seq {|seq_inv:=fun tr _ => forall post (UnqPost : tree_item_determined tg post tr), reach p0 (item_perm_at_loc post z)|}
       tr cids evts tr' cids'.
 Proof.
   pose proof (bor_local_seq_always_contains Ex Seq) as AllEx.
-  pose proof (seq_always_merge AllEx (bor_local_seq_always_unique Ex Unq eq_refl AllEx)) as AllExUnq.
+  pose proof (seq_always_merge AllEx (bor_local_seq_always_determined Ex Unq eq_refl AllEx)) as AllExUnq.
   eapply seq_always_build_forward; [| |exact AllExUnq].
-  + move=> ? Unq'. pose proof (tree_unique_unify Ex Unq Unq'); subst. assumption.
+  + move=> ? Unq'. pose proof (tree_determined_unify Ex Unq Unq'); subst. assumption.
   + clear; simpl; move=> ????? Step [Ex [?[Unq _]]] Reach.
     move=> ? Unq'.
     eapply bor_local_step_preserves_backward_reach; eauto.
@@ -679,24 +679,24 @@ Qed.
 Lemma bor_local_seq_always_protected_freeze_like
   {tg tr tr' cids cids' pre evts cid z}
   (Ex : tree_contains tg tr)
-  (Unq : tree_unique tg pre tr)
+  (Unq : tree_item_determined tg pre tr)
   (Prot : protector_is_for_call cid (iprot pre))
   (Reach : freeze_like (item_perm_at_loc pre z))
   (Seq : bor_local_seq {|seq_inv:=fun _ cids => call_is_active cid cids|} tr cids evts tr' cids')
-  : bor_local_seq {|seq_inv:=fun tr _ => forall post (UnqPost : tree_unique tg post tr), protector_is_for_call cid (iprot post) /\ freeze_like (item_perm_at_loc post z)|}
+  : bor_local_seq {|seq_inv:=fun tr _ => forall post (UnqPost : tree_item_determined tg post tr), protector_is_for_call cid (iprot post) /\ freeze_like (item_perm_at_loc post z)|}
       tr cids evts tr' cids'.
 Proof.
   pose proof (bor_local_seq_always_contains Ex (bor_local_seq_forget Seq)) as AllEx.
-  pose proof (seq_always_merge Seq (seq_always_merge AllEx (bor_local_seq_always_unique Ex Unq eq_refl AllEx))) as AllExUnqProt.
+  pose proof (seq_always_merge Seq (seq_always_merge AllEx (bor_local_seq_always_determined Ex Unq eq_refl AllEx))) as AllExUnqProt.
   eapply seq_always_build_forward; [| |exact AllExUnqProt].
-  + move=> ? Unq'. pose proof (tree_unique_unify Ex Unq Unq'); subst. split; assumption.
+  + move=> ? Unq'. pose proof (tree_determined_unify Ex Unq Unq'); subst. split; assumption.
   + clear; simpl; move=> ???? evt Step [Prot [Ex [? [Unq _]]]] Reach.
     move=> ? Unq'.
     destruct (Reach _ Unq) as [SameProt FrzLike].
     split.
     * pose proof (bor_local_step_preserves_contains Ex Step) as Ex'.
-      destruct (bor_local_step_preserves_unique_easy Ex Unq Step) as [x [Unqx Protx]].
-      pose proof (tree_unique_unify Ex' Unq' Unqx); subst.
+      destruct (bor_local_step_preserves_determined_easy Ex Unq Step) as [x [Unqx Protx]].
+      pose proof (tree_determined_unify Ex' Unq' Unqx); subst.
       destruct evt; rewrite <- Protx; assumption.
     * eapply bor_local_step_preserves_protected_freeze_like; eauto.
       exists cid; split; assumption.
@@ -705,10 +705,10 @@ Qed.
 Lemma bor_local_seq_last_backward_reach
   {tg tr tr' cids cids' pre evts p0 z}
   (Ex : tree_contains tg tr)
-  (Unq : tree_unique tg pre tr)
+  (Unq : tree_item_determined tg pre tr)
   (Reach : reach p0 (item_perm_at_loc pre z))
   (Seq : bor_local_seq {|seq_inv:=fun _ _ => True|} tr cids evts tr' cids')
-  : forall post (UnqPost : tree_unique tg post tr'), reach p0 (item_perm_at_loc post z).
+  : forall post (UnqPost : tree_item_determined tg post tr'), reach p0 (item_perm_at_loc post z).
 Proof.
   pose proof (seq_always_destruct_last (bor_local_seq_always_backward_reach Ex Unq Reach Seq)).
   assumption.
@@ -717,11 +717,11 @@ Qed.
 Lemma bor_local_seq_last_protected_freeze_like
   {tg tr tr' cids cids' pre evts cid z}
   (Ex : tree_contains tg tr)
-  (Unq : tree_unique tg pre tr)
+  (Unq : tree_item_determined tg pre tr)
   (Prot : protector_is_for_call cid (iprot pre))
   (FrzLike : freeze_like (item_perm_at_loc pre z))
   (Seq : bor_local_seq {|seq_inv:=fun _ cids => call_is_active cid cids|} tr cids evts tr' cids')
-  : forall post (UnqPost : tree_unique tg post tr'), protector_is_for_call cid (iprot post) /\ freeze_like (item_perm_at_loc post z).
+  : forall post (UnqPost : tree_item_determined tg post tr'), protector_is_for_call cid (iprot post) /\ freeze_like (item_perm_at_loc post z).
 Proof.
   pose proof (seq_always_destruct_last (bor_local_seq_always_protected_freeze_like Ex Unq Prot FrzLike Seq)).
   assumption.
@@ -730,16 +730,16 @@ Qed.
 Lemma bor_local_seq_always_forward_unreach
   {tg tr tr' cids cids' pre evts p0 z}
   (Ex : tree_contains tg tr)
-  (Unq : tree_unique tg pre tr)
+  (Unq : tree_item_determined tg pre tr)
   (Unreach : ~reach (item_perm_at_loc pre z) p0)
   (Seq : bor_local_seq {|seq_inv:=fun _ _ => True|} tr cids evts tr' cids')
-  : bor_local_seq {|seq_inv:=fun tr _ => forall post (UnqPost : tree_unique tg post tr), ~reach (item_perm_at_loc post z) p0|}
+  : bor_local_seq {|seq_inv:=fun tr _ => forall post (UnqPost : tree_item_determined tg post tr), ~reach (item_perm_at_loc post z) p0|}
       tr cids evts tr' cids'.
 Proof.
   pose proof (bor_local_seq_always_contains Ex Seq) as AllEx.
-  pose proof (seq_always_merge AllEx (bor_local_seq_always_unique Ex Unq eq_refl AllEx)) as AllExUnq.
+  pose proof (seq_always_merge AllEx (bor_local_seq_always_determined Ex Unq eq_refl AllEx)) as AllExUnq.
   eapply seq_always_build_forward; [| |exact AllExUnq].
-  + move=> ? Unq'. pose proof (tree_unique_unify Ex Unq Unq'); subst. assumption.
+  + move=> ? Unq'. pose proof (tree_determined_unify Ex Unq Unq'); subst. assumption.
   + clear; move=> ????? Step [Ex [?[Unq _]]] Reach.
     move=> ? Unq'.
     eapply bor_local_step_preserves_forward_unreach; eauto.
@@ -748,10 +748,10 @@ Qed.
 Lemma bor_local_seq_last_forward_unreach
   {tg tr tr' cids cids' pre evts p0 z}
   (Ex : tree_contains tg tr)
-  (Unq : tree_unique tg pre tr)
+  (Unq : tree_item_determined tg pre tr)
   (Unreach : ~reach (item_perm_at_loc pre z) p0)
   (Seq : bor_local_seq {|seq_inv:=fun _ _ => True|} tr cids evts tr' cids')
-  : forall post (UnqPost : tree_unique tg post tr'), ~reach (item_perm_at_loc post z) p0.
+  : forall post (UnqPost : tree_item_determined tg post tr'), ~reach (item_perm_at_loc post z) p0.
 Proof.
   pose proof (seq_always_destruct_last (bor_local_seq_always_forward_unreach Ex Unq Unreach Seq)).
   assumption.
@@ -804,17 +804,17 @@ Qed.
 Lemma memory_access_preserves_perminit
   {access_tag affected_tag pre tr post tr' kind cids range z zpre zpost}
   (ExAff : tree_contains affected_tag tr)
-  (UnqAff : tree_unique affected_tag pre tr)
+  (UnqAff : tree_item_determined affected_tag pre tr)
   (ExAcc : tree_contains access_tag tr)
   (Access : memory_access kind cids access_tag range tr = Some tr')
-  (UnqAff' : tree_unique affected_tag post tr')
+  (UnqAff' : tree_item_determined affected_tag post tr')
   (ItemPre : item_lazy_perm_at_loc pre z = zpre)
   (ItemPost : item_lazy_perm_at_loc post z = zpost)
   (Init : initialized zpre = PermInit)
   : initialized zpost = PermInit.
 Proof.
   destruct (apply_access_spec_per_node ExAff UnqAff Access) as [post' [PostSpec [ExPost UnqPost]]].
-  pose proof (tree_unique_unify ExPost UnqPost UnqAff'); subst.
+  pose proof (tree_determined_unify ExPost UnqPost UnqAff'); subst.
   generalize dependent post.
   generalize dependent pre.
   clear. move=> pre _ Init post _ Access _.
@@ -846,19 +846,19 @@ Qed.
 Lemma memory_access_child_produces_perminit
   {access_tag affected_tag pre tr post tr' kind cids range z zpre zpost}
   (ExAff : tree_contains affected_tag tr)
-  (UnqAff : tree_unique affected_tag pre tr)
+  (UnqAff : tree_item_determined affected_tag pre tr)
   (ExAcc : tree_contains access_tag tr)
   (Access : memory_access kind cids access_tag range tr = Some tr')
   (Rel : ParentChildIn affected_tag access_tag tr)
   (WithinRange : range'_contains range z)
-  (UnqAff' : tree_unique affected_tag post tr')
+  (UnqAff' : tree_item_determined affected_tag post tr')
   (ItemPre : item_lazy_perm_at_loc pre z = zpre)
   (ItemPost : item_lazy_perm_at_loc post z = zpost)
   : initialized zpost = PermInit.
 Proof.
   destruct (apply_access_spec_per_node ExAff UnqAff Access) as [post' [PostSpec [ExPost UnqPost]]].
-  pose proof (tree_unique_unify ExPost UnqPost UnqAff'); subst.
-  rewrite (tree_unique_specifies_tag _ _ _ ExAff UnqAff) in PostSpec.
+  pose proof (tree_determined_unify ExPost UnqPost UnqAff'); subst.
+  rewrite (tree_determined_specifies_tag _ _ _ ExAff UnqAff) in PostSpec.
   unfold rel_dec in PostSpec.
   destruct (decide (ParentChildIn affected_tag access_tag tr)); [|contradiction].
   destruct (decide (ParentChildIn access_tag affected_tag tr)).
@@ -879,12 +879,12 @@ Qed.
 Lemma bor_local_step_preserves_perminit
   {affected_tag tr cids evt tr' cids' pre z zpre}
   (Ex : tree_contains affected_tag tr)
-  (Unq : tree_unique affected_tag pre tr)
+  (Unq : tree_item_determined affected_tag pre tr)
   (ItemPre : item_lazy_perm_at_loc pre z = zpre)
   (Initialized : initialized zpre = PermInit)
   (Step : bor_local_step tr cids evt tr' cids')
   : forall post,
-    tree_unique affected_tag post tr' ->
+    tree_item_determined affected_tag post tr' ->
     initialized (item_lazy_perm_at_loc post z) = PermInit.
 Proof.
   move=> post Unq'.
@@ -898,26 +898,26 @@ Proof.
     + reflexivity.
     + reflexivity.
     + exact Initialized.
-  - pose proof (tree_unique_unify Ex Unq Unq'); subst.
+  - pose proof (tree_determined_unify Ex Unq Unq'); subst.
     assumption.
-  - pose proof (tree_unique_unify Ex Unq Unq'); subst.
+  - pose proof (tree_determined_unify Ex Unq Unq'); subst.
     assumption.
   - assert (affected_tag ≠ tg) as Ne by (intro; subst; contradiction).
-    pose proof (create_child_preserves_unique _ _ _ _ _ _ _ _ Ne Unq RETAG_EFFECT) as UnqPost.
+    pose proof (create_child_preserves_determined _ _ _ _ _ _ _ _ Ne Unq RETAG_EFFECT) as UnqPost.
     pose proof (insertion_preserves_tags Ex RETAG_EFFECT) as Ex'.
-    pose proof (tree_unique_unify Ex' UnqPost Unq'); subst.
+    pose proof (tree_determined_unify Ex' UnqPost Unq'); subst.
     assumption.
 Qed.
 
 Lemma bor_local_step_child_produces_perminit
   {access_tag affected_tag pre tr tr' kind cids cids' z range}
   (ExAff : tree_contains affected_tag tr)
-  (UnqAff : tree_unique affected_tag pre tr)
+  (UnqAff : tree_item_determined affected_tag pre tr)
   (Rel : ParentChildIn affected_tag access_tag tr)
   (WithinRange : range'_contains range z)
   (Step : bor_local_step tr cids (AccessBLEvt kind access_tag range) tr' cids')
   : forall post,
-    tree_unique affected_tag post tr' ->
+    tree_item_determined affected_tag post tr' ->
     initialized (item_lazy_perm_at_loc post z) = PermInit.
 Proof.
   inversion Step; subst.
@@ -930,20 +930,20 @@ Qed.
 Lemma bor_local_seq_always_perminit
   {affected_tag tr tr' cids cids' evts pre z}
   (Ex : tree_contains affected_tag tr)
-  (Unq : tree_unique affected_tag pre tr)
+  (Unq : tree_item_determined affected_tag pre tr)
   (InitPre : initialized (item_lazy_perm_at_loc pre z) = PermInit)
   (Seq : bor_local_seq {|seq_inv:=fun _ _ => True|} tr cids evts tr' cids')
   : bor_local_seq
     {|seq_inv:=fun tr _ =>
       forall it,
-      tree_unique affected_tag it tr ->
+      tree_item_determined affected_tag it tr ->
       initialized (item_lazy_perm_at_loc it z) = PermInit|}
     tr cids evts tr' cids'.
 Proof.
   pose proof (bor_local_seq_always_contains Ex Seq) as SeqEx.
-  pose proof (bor_local_seq_always_unique Ex Unq eq_refl SeqEx) as SeqUnq.
+  pose proof (bor_local_seq_always_determined Ex Unq eq_refl SeqEx) as SeqUnq.
   eapply seq_always_build_forward; simpl; [| |exact (seq_always_merge SeqEx SeqUnq)].
-  - intros pre' Unq'. pose proof (tree_unique_unify Ex Unq Unq'); subst.
+  - intros pre' Unq'. pose proof (tree_determined_unify Ex Unq Unq'); subst.
     assumption.
   - intros ????? Step Inv Init.
     simpl in Inv; destruct Inv as [Exi [?[Unqi ?]]].
@@ -968,10 +968,10 @@ Qed.
 Lemma memory_access_protected_initialized_preserves_active
   {access_tag affected_tag pre tr post tr' kind cids range z zpre zpost}
   (ExAff : tree_contains affected_tag tr)
-  (UnqAff : tree_unique affected_tag pre tr)
+  (UnqAff : tree_item_determined affected_tag pre tr)
   (ExAcc : tree_contains access_tag tr)
   (Access : memory_access kind cids access_tag range tr = Some tr')
-  (UnqAff' : tree_unique affected_tag post tr')
+  (UnqAff' : tree_item_determined affected_tag post tr')
   (Prot : protector_is_active (iprot pre) cids)
   (ItemPre : item_lazy_perm_at_loc pre z = zpre)
   (ItemPost : item_lazy_perm_at_loc post z = zpost)
@@ -979,7 +979,7 @@ Lemma memory_access_protected_initialized_preserves_active
   : perm zpre = Active -> perm zpost = Active.
 Proof.
   destruct (apply_access_spec_per_node ExAff UnqAff Access) as [post' [PostSpec [ExPost UnqPost]]].
-  pose proof (tree_unique_unify ExPost UnqPost UnqAff'); subst.
+  pose proof (tree_determined_unify ExPost UnqPost UnqAff'); subst.
   (* now it's just bruteforce case analysis *)
   generalize dependent post.
   generalize dependent pre.
@@ -1000,45 +1000,45 @@ Qed.
 Lemma protected_during_step_stays_active
   {affected_tag tr cids evt tr' cids' pre z zpre}
   (Ex : tree_contains affected_tag tr)
-  (Unq : tree_unique affected_tag pre tr)
+  (Unq : tree_item_determined affected_tag pre tr)
   (Prot : protector_is_active (iprot pre) cids)
   (ItemPre : item_lazy_perm_at_loc pre z = zpre)
   (Init : initialized zpre = PermInit)
   (ActPre : perm zpre = Active)
   (Step : bor_local_step tr cids evt tr' cids')
-  : forall post, tree_unique affected_tag post tr' -> item_perm_at_loc post z = Active.
+  : forall post, tree_item_determined affected_tag post tr' -> item_perm_at_loc post z = Active.
 Proof.
   move=> ? Unq'.
   inversion Step as [???? EXISTS_TAG ACC| | |?? tg???? FRESH_CHILD ? RETAG_EFFECT]; subst.
   - apply (memory_access_protected_initialized_preserves_active Ex Unq EXISTS_TAG ACC Unq' Prot eq_refl eq_refl Init ActPre).
-  - rewrite <- (tree_unique_unify Ex Unq Unq'); tauto.
-  - rewrite <- (tree_unique_unify Ex Unq Unq'); tauto.
+  - rewrite <- (tree_determined_unify Ex Unq Unq'); tauto.
+  - rewrite <- (tree_determined_unify Ex Unq Unq'); tauto.
   - pose proof (bor_local_step_preserves_contains Ex Step) as ExPost'.
-    pose proof (bor_local_step_preserves_unique_easy Ex Unq Step) as [it' [UnqPost' Eq]]; subst; simpl in UnqPost'.
-    rewrite <- (tree_unique_unify ExPost' UnqPost' Unq'); tauto.
+    pose proof (bor_local_step_preserves_determined_easy Ex Unq Step) as [it' [UnqPost' Eq]]; subst; simpl in UnqPost'.
+    rewrite <- (tree_determined_unify ExPost' UnqPost' Unq'); tauto.
 Qed.
 
 Lemma protected_during_seq_always_stays_active
   {affected_tag tr cids evts tr' cid cids' prot pre z}
   (Ex : tree_contains affected_tag tr)
-  (Unq : tree_unique affected_tag pre tr)
+  (Unq : tree_item_determined affected_tag pre tr)
   (Prot : iprot pre = prot)
   (Call : protector_is_for_call cid prot)
   (StartsActive : item_perm_at_loc pre z = Active)
   (Seq : bor_local_seq
     {|seq_inv:=fun tr cids =>
-      (forall it, tree_unique affected_tag it tr -> initialized (item_lazy_perm_at_loc it z) = PermInit)
+      (forall it, tree_item_determined affected_tag it tr -> initialized (item_lazy_perm_at_loc it z) = PermInit)
       /\ call_is_active cid cids|}
     tr cids evts tr' cids')
   : bor_local_seq
-    {|seq_inv:=fun tr _ => forall it, tree_unique affected_tag it tr -> perm (item_lazy_perm_at_loc it z) = Active|}
+    {|seq_inv:=fun tr _ => forall it, tree_item_determined affected_tag it tr -> perm (item_lazy_perm_at_loc it z) = Active|}
     tr cids evts tr' cids'.
 Proof.
   pose proof (bor_local_seq_always_contains Ex (bor_local_seq_forget Seq)) as AllEx.
-  pose proof (bor_local_seq_always_unique Ex Unq Prot AllEx) as AllUnq.
+  pose proof (bor_local_seq_always_determined Ex Unq Prot AllEx) as AllUnq.
   pose proof (seq_always_merge AllEx (seq_always_merge Seq AllUnq)) as AllExUnqInitProt.
   eapply seq_always_build_forward; [| |exact AllExUnqInitProt].
-  + move=> it Unq'. pose proof (tree_unique_unify Ex Unq Unq'); subst. assumption.
+  + move=> it Unq'. pose proof (tree_determined_unify Ex Unq Unq'); subst. assumption.
   + generalize Call; clear; simpl; move=> Call ????? Step [Ex [[Init CallAct] [?[Unq ProtEq]]]] Act.
     move=> ? Unq'.
     subst.
@@ -1049,16 +1049,16 @@ Qed.
 Lemma protected_during_seq_last_stays_active
   {affected_tag tr cids evts tr' cids' cid prot pre z}
   (Ex : tree_contains affected_tag tr)
-  (Unq : tree_unique affected_tag pre tr)
+  (Unq : tree_item_determined affected_tag pre tr)
   (Prot : iprot pre = prot)
   (Call : protector_is_for_call cid prot)
   (StartsActive : item_perm_at_loc pre z = Active)
   (Seq : bor_local_seq
     {|seq_inv:=fun tr cids =>
-      (forall it, tree_unique affected_tag it tr -> initialized (item_lazy_perm_at_loc it z) = PermInit)
+      (forall it, tree_item_determined affected_tag it tr -> initialized (item_lazy_perm_at_loc it z) = PermInit)
       /\ call_is_active cid cids|}
     tr cids evts tr' cids')
-  : forall post, tree_unique affected_tag post tr' -> perm (item_lazy_perm_at_loc post z) = Active.
+  : forall post, tree_item_determined affected_tag post tr' -> perm (item_lazy_perm_at_loc post z) = Active.
 Proof.
   pose proof (seq_always_destruct_last (protected_during_seq_always_stays_active Ex Unq Prot Call StartsActive Seq)).
   assumption.
@@ -1080,10 +1080,10 @@ Qed.
 Lemma memory_access_protected_initialized_preserves_nondis
   {access_tag affected_tag pre tr post tr' kind cids range z zpre zpost}
   (ExAff : tree_contains affected_tag tr)
-  (UnqAff : tree_unique affected_tag pre tr)
+  (UnqAff : tree_item_determined affected_tag pre tr)
   (ExAcc : tree_contains access_tag tr)
   (Access : memory_access kind cids access_tag range tr = Some tr')
-  (UnqAff' : tree_unique affected_tag post tr')
+  (UnqAff' : tree_item_determined affected_tag post tr')
   (Prot : protector_is_active (iprot pre) cids)
   (ItemPre : item_lazy_perm_at_loc pre z = zpre)
   (ItemPost : item_lazy_perm_at_loc post z = zpost)
@@ -1091,7 +1091,7 @@ Lemma memory_access_protected_initialized_preserves_nondis
   : ~reach Disabled (perm zpre) -> ~reach Disabled (perm zpost).
 Proof.
   destruct (apply_access_spec_per_node ExAff UnqAff Access) as [post' [PostSpec [ExPost UnqPost]]].
-  pose proof (tree_unique_unify ExPost UnqPost UnqAff'); subst.
+  pose proof (tree_determined_unify ExPost UnqPost UnqAff'); subst.
   (* now it's just bruteforce case analysis *)
   generalize dependent post.
   generalize dependent pre.
@@ -1112,45 +1112,45 @@ Qed.
 Lemma protected_during_step_stays_nondis
   {affected_tag tr cids evt tr' cids' pre z zpre}
   (Ex : tree_contains affected_tag tr)
-  (Unq : tree_unique affected_tag pre tr)
+  (Unq : tree_item_determined affected_tag pre tr)
   (Prot : protector_is_active (iprot pre) cids)
   (ItemPre : item_lazy_perm_at_loc pre z = zpre)
   (Init : initialized zpre = PermInit)
   (NonDisPre : ~reach Disabled (perm zpre))
   (Step : bor_local_step tr cids evt tr' cids')
-  : forall post, tree_unique affected_tag post tr' -> ~reach Disabled (item_perm_at_loc post z).
+  : forall post, tree_item_determined affected_tag post tr' -> ~reach Disabled (item_perm_at_loc post z).
 Proof.
   move=> ? Unq'.
   inversion Step as [???? EXISTS_TAG ACC| | |?? tg???? FRESH_CHILD ? RETAG_EFFECT]; subst.
   - apply (memory_access_protected_initialized_preserves_nondis Ex Unq EXISTS_TAG ACC Unq' Prot eq_refl eq_refl Init NonDisPre).
-  - rewrite <- (tree_unique_unify Ex Unq Unq'); tauto.
-  - rewrite <- (tree_unique_unify Ex Unq Unq'); tauto.
+  - rewrite <- (tree_determined_unify Ex Unq Unq'); tauto.
+  - rewrite <- (tree_determined_unify Ex Unq Unq'); tauto.
   - pose proof (bor_local_step_preserves_contains Ex Step) as ExPost'.
-    pose proof (bor_local_step_preserves_unique_easy Ex Unq Step) as [it' [UnqPost' Eq]]; subst; simpl in UnqPost'.
-    rewrite <- (tree_unique_unify ExPost' UnqPost' Unq'); tauto.
+    pose proof (bor_local_step_preserves_determined_easy Ex Unq Step) as [it' [UnqPost' Eq]]; subst; simpl in UnqPost'.
+    rewrite <- (tree_determined_unify ExPost' UnqPost' Unq'); tauto.
 Qed.
 
 Lemma protected_during_seq_always_stays_nondis
   {affected_tag tr cids evts tr' cid cids' prot pre z}
   (Ex : tree_contains affected_tag tr)
-  (Unq : tree_unique affected_tag pre tr)
+  (Unq : tree_item_determined affected_tag pre tr)
   (Prot : iprot pre = prot)
   (Call : protector_is_for_call cid prot)
   (StartsNonDis : ~reach Disabled (item_perm_at_loc pre z))
   (Seq : bor_local_seq
     {|seq_inv:=fun tr cids =>
-      (forall it, tree_unique affected_tag it tr -> initialized (item_lazy_perm_at_loc it z) = PermInit)
+      (forall it, tree_item_determined affected_tag it tr -> initialized (item_lazy_perm_at_loc it z) = PermInit)
       /\ call_is_active cid cids|}
     tr cids evts tr' cids')
   : bor_local_seq
-    {|seq_inv:=fun tr _ => forall it, tree_unique affected_tag it tr -> ~reach Disabled (perm (item_lazy_perm_at_loc it z))|}
+    {|seq_inv:=fun tr _ => forall it, tree_item_determined affected_tag it tr -> ~reach Disabled (perm (item_lazy_perm_at_loc it z))|}
     tr cids evts tr' cids'.
 Proof.
   pose proof (bor_local_seq_always_contains Ex (bor_local_seq_forget Seq)) as AllEx.
-  pose proof (bor_local_seq_always_unique Ex Unq Prot AllEx) as AllUnq.
+  pose proof (bor_local_seq_always_determined Ex Unq Prot AllEx) as AllUnq.
   pose proof (seq_always_merge AllEx (seq_always_merge Seq AllUnq)) as AllExUnqInitProt.
   eapply seq_always_build_forward; [| |exact AllExUnqInitProt].
-  + move=> it Unq'. pose proof (tree_unique_unify Ex Unq Unq'); subst. assumption.
+  + move=> it Unq'. pose proof (tree_determined_unify Ex Unq Unq'); subst. assumption.
   + generalize Call; clear; simpl; move=> Call ????? Step [Ex [[Init CallAct] [?[Unq ProtEq]]]] Act.
     move=> ? Unq'.
     subst.
@@ -1161,16 +1161,16 @@ Qed.
 Lemma protected_during_seq_last_stays_nondis
   {affected_tag tr cids evts tr' cids' cid prot pre z}
   (Ex : tree_contains affected_tag tr)
-  (Unq : tree_unique affected_tag pre tr)
+  (Unq : tree_item_determined affected_tag pre tr)
   (Prot : iprot pre = prot)
   (Call : protector_is_for_call cid prot)
   (StartsNonDis : ~reach Disabled (item_perm_at_loc pre z))
   (Seq : bor_local_seq
     {|seq_inv:=fun tr cids =>
-      (forall it, tree_unique affected_tag it tr -> initialized (item_lazy_perm_at_loc it z) = PermInit)
+      (forall it, tree_item_determined affected_tag it tr -> initialized (item_lazy_perm_at_loc it z) = PermInit)
       /\ call_is_active cid cids|}
     tr cids evts tr' cids')
-  : forall post, tree_unique affected_tag post tr' -> ~reach Disabled (perm (item_lazy_perm_at_loc post z)).
+  : forall post, tree_item_determined affected_tag post tr' -> ~reach Disabled (perm (item_lazy_perm_at_loc post z)).
 Proof.
   pose proof (seq_always_destruct_last (protected_during_seq_always_stays_nondis Ex Unq Prot Call StartsNonDis Seq)).
   assumption.
@@ -1180,7 +1180,7 @@ Qed.
 
 == Preservation lemmas ==
 [X] contains
-[X] unique (quantified)
+[X] determined (quantified)
 [X] reach, unreach
 [X] when protected: stays active, stays frozen
 [X] stays initialized
