theories/tree_borrows/tree.v
@@ -103,6 +103,9 @@ Definition exists_node {X} (prop:Tprop X) (tr:tree X) := fold_nodes False (fun d
 Global Instance exists_node_dec {X} prop (tr:tree X) : (forall x, Decision (prop x)) -> Decision (exists_node prop tr).
 Proof. intro. induction tr; solve_decision. Qed.
 
+Definition count_nodes {X} (prop:X -> bool) :=
+  fold_nodes 0 (fun data lt rt => (if prop data then 1 else 0) + lt + rt).
+
 Definition exists_strict_child {X} (prop:Tprop X)
   : Tprop (tbranch X) := fun '(_, _, child) => exists_node prop child.
 Global Instance exists_strict_child_dec {X} prop (tr:tbranch X) :
